theories/Core/Semantic/PER.v
@@ -1,1 +1,1 @@
-From Mcltt Require Export PERBasicLemmas PERDefinitions.
+From Mcltt Require Export PERDefinitions PERLemmas.
