theories/Core/Semantic/PERLemmas.v
@@ -1,0 +1,119 @@
+From Coq Require Import Lia PeanoNat Relation_Definitions RelationClasses.
+From Mcltt Require Import Axioms Base Evaluation LibTactics PERDefinitions.
+From Mcltt Require Export PERBasicLemmas.
+Import Domain_Notations.
+
+Lemma per_ctx_env_right_irrel : forall Γ Δ Δ' R R',
+    {{ DF Γ ≈ Δ ∈ per_ctx_env ↘ R }} ->
+    {{ DF Γ ≈ Δ' ∈ per_ctx_env ↘ R' }} ->
+    R = R'.
+Proof.
+  intros * Horig; gen Δ' R'.
+  induction Horig; intros * Hright;
+    try solve [inversion Hright; congruence].
+  subst.
+  inversion_clear Hright.
+  specialize (IHHorig _ _ equiv_Γ_Γ'0).
+  subst.
+  enough (head_rel = head_rel0) by (subst; easy).
+  extensionality p.
+  extensionality p'.
+  extensionality equiv_p_p'.
+  unfold rel_typ in *.
+  destruct_rel_mod_eval.
+  per_univ_elem_irrel_rewrite.
+  congruence.
+Qed.
+
+Lemma per_ctx_env_sym : forall Γ Δ R,
+    {{ DF Γ ≈ Δ ∈ per_ctx_env ↘ R }} ->
+    {{ DF Δ ≈ Γ ∈ per_ctx_env ↘ R }} /\ (forall o p, {{ Dom o ≈ p ∈ R }} -> {{ Dom p ≈ o ∈ R }}).
+Proof with solve [eauto].
+  simpl.
+  induction 1; firstorder; try solve [econstructor; eauto]; unfold rel_typ in *.
+  - econstructor; eauto; firstorder.
+    assert (tail_rel p' p) by eauto.
+    assert (tail_rel p p) by (etransitivity; eauto).
+    destruct_rel_mod_eval.
+    per_univ_elem_irrel_rewrite.
+    econstructor; eauto.
+    apply per_univ_elem_sym...
+  - subst.
+    firstorder.
+    assert (tail_rel d{{{ p ↯ }}} d{{{ o ↯ }}}) by (unfold Symmetric in *; eauto).
+    assert (tail_rel d{{{ p ↯ }}} d{{{ p ↯ }}}) by (etransitivity; eauto).
+    destruct_rel_mod_eval.
+    eexists.
+    per_univ_elem_irrel_rewrite.
+    eapply per_univ_elem_sym...
+Qed.
+
+Lemma per_ctx_env_left_irrel : forall Γ Γ' Δ R R',
+    {{ DF Γ ≈ Δ ∈ per_ctx_env ↘ R }} ->
+    {{ DF Γ' ≈ Δ ∈ per_ctx_env ↘ R' }} ->
+    R = R'.
+Proof.
+  intros * []%per_ctx_env_sym []%per_ctx_env_sym.
+  eauto using per_ctx_env_right_irrel.
+Qed.
+
+Lemma per_ctx_env_cross_irrel : forall Γ Δ Δ' R R',
+    {{ DF Γ ≈ Δ ∈ per_ctx_env ↘ R }} ->
+    {{ DF Δ' ≈ Γ ∈ per_ctx_env ↘ R' }} ->
+    R = R'.
+Proof.
+  intros * ? []%per_ctx_env_sym.
+  eauto using per_ctx_env_right_irrel.
+Qed.
+
+Ltac do_per_ctx_env_irrel_rewrite1 :=
+  match goal with
+    | H1 : {{ DF ~?Γ ≈ ~_ ∈ per_ctx_env ↘ ?R1 }},
+        H2 : {{ DF ~?Γ ≈ ~_ ∈ per_ctx_env ↘ ?R2 }} |- _ =>
+        clean replace R2 with R1 by (eauto using per_ctx_env_right_irrel)
+    | H1 : {{ DF ~_ ≈ ~?Δ ∈ per_ctx_env ↘ ?R1 }},
+        H2 : {{ DF ~_ ≈ ~?Δ ∈ per_ctx_env ↘ ?R2 }} |- _ =>
+        clean replace R2 with R1 by (eauto using per_ctx_env_left_irrel)
+    | H1 : {{ DF ~?Γ ≈ ~_ ∈ per_ctx_env ↘ ?R1 }},
+        H2 : {{ DF ~_ ≈ ~?Γ ∈ per_ctx_env ↘ ?R2 }} |- _ =>
+        (* Order matters less here as H1 and H2 cannot be exchanged *)
+        clean replace R2 with R1 by (symmetry; eauto using per_ctx_env_cross_irrel)
+    end.
+
+Ltac do_per_ctx_env_irrel_rewrite :=
+  repeat do_per_ctx_env_irrel_rewrite1.
+
+Ltac per_ctx_env_irrel_rewrite :=
+  functional_eval_rewrite_clear;
+  do_per_ctx_env_irrel_rewrite;
+  clear_dups.
+
+Lemma per_ctx_env_trans : forall Γ1 Γ2 R,
+    {{ DF Γ1 ≈ Γ2 ∈ per_ctx_env ↘ R }} ->
+    forall Γ3,
+      {{ DF Γ2 ≈ Γ3 ∈ per_ctx_env ↘ R }} ->
+      {{ DF Γ1 ≈ Γ3 ∈ per_ctx_env ↘ R }} /\ (forall p1 p2 p3, {{ Dom p1 ≈ p2 ∈ R }} -> {{ Dom p2 ≈ p3 ∈ R }} -> {{ Dom p1 ≈ p3 ∈ R }}).
+Proof with solve [eauto].
+  simpl.
+  induction 1; intros * HTrans23; inversion HTrans23; subst; eauto.
+  per_ctx_env_irrel_rewrite.
+  rename tail_rel0 into tail_rel.
+  split.
+  - econstructor; eauto.
+    + eapply IHper_ctx_env...
+    + unfold rel_typ in *.
+      intros.
+      assert (tail_rel p p) by (etransitivity; [ | symmetry]; eassumption).
+      destruct_rel_mod_eval.
+      econstructor; eauto.
+      per_univ_elem_irrel_rewrite.
+      eapply proj1, per_univ_elem_trans; [|eassumption]...
+  - intros * [] [].
+    specialize (IHper_ctx_env _ equiv_Γ_Γ'0) as [].
+    assert (tail_rel d{{{ p1 ↯ }}} d{{{ p3 ↯ }}}) by eauto.
+    eexists.
+    unfold rel_typ in *.
+    destruct_rel_mod_eval.
+    per_univ_elem_irrel_rewrite.
+    eapply per_univ_elem_trans...
+Qed.
